src/PushButtonSynthesis/SaturatedSolinas.v
@@ -32,6 +32,7 @@ Require Import Crypto.PushButtonSynthesis.ReificationCache.
 Require Import Crypto.PushButtonSynthesis.Primitives.
 Require Import Crypto.PushButtonSynthesis.SaturatedSolinasReificationCache.
 Require Import Crypto.Assembly.Equivalence.
+Require Import Crypto.Assembly.Symbolic.
 Import ListNotations.
 Local Open Scope string_scope. Local Open Scope Z_scope. Local Open Scope list_scope. Local Open Scope bool_scope.
 
@@ -83,6 +84,7 @@ Section __.
           {widen_carry : widen_carry_opt}
           (widen_bytes : widen_bytes_opt := true) (* true, because we don't allow byte-sized things anyway, so we should not expect carries to be widened to byte-size when emitting C code *)
           {assembly_conventions : assembly_conventions_opt}
+          {errules : extra_rewrite_rules}
           {error_on_unused_assembly_functions : error_on_unused_assembly_functions_opt}
           (s : Z)
           (c : list (Z * Z))
